src/Spec/Abstraction.v
@@ -18,11 +18,10 @@ Section Abstraction.
   (* define refinement as transforming an abstract specification to a concrete
   one (a program satisfying the abstract spec should satisfy the concrete spec
   after refinement-preserving compilation) *)
-  (*
   Definition refine_spec
              A T R
-             (spec: Specification A T R AState)
-    : Specification (AState*A) T R CState :=
+             (spec: A -> Specification T R AState)
+    : (AState*A) -> Specification T R CState :=
     fun '(s, a) cs =>
       {| pre := absr s cs tt /\
                 (spec a s).(pre);
@@ -32,7 +31,6 @@ Section Abstraction.
          alternate := fun cs' r =>
                         exists s', absr s' cs' tt /\
                               (spec a s).(alternate) s' r; |}.
-   *)
 
   Section Dynamics.
     Context C_Op (c_sem: Dynamics C_Op CState).
